common/ExposedSimulations.v
@@ -283,9 +283,6 @@ Section ExposingMemory.
         Injfsim_order_wf: well_founded Injorder;
         Injfsim_match_meminj: forall i f s1 s2, Injmatch_states i f s1 s2 ->  Mem.inject f (get_mem1 s1) (get_mem2 s2);
         Injfsim_match_full: forall i f s1 s2, Injmatch_states i f s1 s2 ->  injection_full f (get_mem1 s1);
-        (*    fsim_match_initial_states:
-      forall s1 m1 f m2, initial_state L1 (s1,m1) -> Mem.inject f m1 m2 ->
-      exists i, exists s2, initial_state L2 (s2,m2) /\ match_states i f (s1,m1) (s2,m2);*)
         Injfsim_match_initial_states:
           forall s1, initial_state L1 s1 -> 
                 exists i f s2, initial_state L2 s2 /\ Injmatch_states i f s1 s2;
